Added associativity

icounter.fst
@@ -27,11 +27,15 @@ let rec lemma1 tr s1 =
      let s2 = app_op s1 op in
      lemma1 ops s2
 
+val lemma2 : l:s -> a:s{a >= l} -> b:s{b >= l} -> c:s{c >= l} 
+           -> Lemma (ensures ((a + b - l) + c - l) = (a + (b + c - l) - l))
+let lemma2 l a b c = ()
+
 val merge : h:history s o{wellformed h}
           -> a:history s o{hbeq h a}
           -> b:history s o{hbeq h b}
           -> l:history s o{lca h a b = [l]}
-          -> s
+          -> m:history s o
 let merge h a b l = 
   History.lemma1 h;
   assert (wellformed a);
@@ -43,23 +47,43 @@ let merge h a b l =
   lemma1 tr (get_state l);
   assert (get_state a >= get_state l);
 
-  get_state a + get_state b - get_state l
+  (HistLeaf 0 (get_state a + get_state b - get_state l))
 
 val commutativity : h:history s o{wellformed h}
                   -> a:history s o{hbeq h a}
                   -> b:history s o{hbeq h b}
                   -> l:history s o{lca h a b = [l] /\ lca h b a = [l]}
-                  -> Lemma (ensures (merge h a b l = merge h b a l))
+                  -> Lemma (ensures (get_state (merge h a b l) = get_state (merge h b a l)))
 let commutativity h a b l = ()
 
 val idempotence : h:history s o{wellformed h}
                 -> a:history s o{hbeq h a}
                 -> Lemma (requires (lca h a a = [a]))
-                        (ensures (merge h a a a = get_state a))
+                        (ensures  (get_state (merge h a a a) = get_state a))
 let idempotence h a = ()
+
+val associativity : h:history s o{wellformed h} 
+                  -> a:history s o{hbeq h a} 
+                  -> b:history s o{hbeq h b} 
+                  -> c:history s o{hbeq h c}
+                  -> l:history s o{lca h a b = [l] /\ lca h b c = [l] }
+                  -> Lemma (requires (hbeq h (merge h a b l)) /\ (hbeq h (merge h b c l)) /\ 
+                                    (lca h (merge h a b l) c = [l]) /\ (lca h a (merge h b c l) = [l])) 
+                          (ensures  (merge h (merge h a b l) c l) = (merge h a (merge h b c l) l))
+
+let associativity h a b c l = 
+    History.lemma1 h;
+    let tr_a = get_trace l a in
+    let tr_b = get_trace l b in
+    let tr_c = get_trace l c in
+    lemma1 tr_a (get_state l);
+    lemma1 tr_b (get_state l);
+    lemma1 tr_c (get_state l);
+    lemma2 (get_state l) (get_state a) (get_state b) (get_state c); ()
 
 instance _ : mrdt s o icounter = {
   History.merge = merge;
   History.commutativity = commutativity;
-  History.idempotence = idempotence
+  History.idempotence = idempotence;
+  History.associativity = associativity
 }
